add reachable route target provider

rocq/theories/TypeSystem/TypeSafetyDirectCallRoute.v
@@ -1113,6 +1113,37 @@ Definition store_safe_synthetic_direct_call_ready_exact_body_call_route_reachabl
     store_safe_synthetic_direct_call_ready_exact_body_call_route_package_at
       env fname.
 
+Definition store_safe_synthetic_direct_call_ready_exact_body_call_route_reachable_exact_body_target_provider
+    (base_env : global_env) (base_fname : ident) : Prop :=
+  forall env fname,
+    store_safe_synthetic_direct_call_ready_exact_body_call_route_reachable
+      base_env base_fname env fname ->
+    forall fdef fcall used used' fname_body args_body synthetic_body,
+      In fdef (env_fns env) ->
+      fn_name fdef = fname ->
+      alpha_rename_fn_def used fdef = (fcall, used') ->
+      direct_call_target_expr (fn_body fcall) =
+        Some (fname_body, args_body, synthetic_body) ->
+      direct_call_target_expr (fn_body fcall) =
+        Some (fname_body, args_body, fn_body fcall).
+
+Lemma store_safe_synthetic_direct_call_ready_exact_body_call_route_reachable_exact_body_target_provider_of_all :
+  (forall env fname fdef fcall used used' fname_body args_body synthetic_body,
+    In fdef (env_fns env) ->
+    fn_name fdef = fname ->
+    alpha_rename_fn_def used fdef = (fcall, used') ->
+    direct_call_target_expr (fn_body fcall) =
+      Some (fname_body, args_body, synthetic_body) ->
+    direct_call_target_expr (fn_body fcall) =
+      Some (fname_body, args_body, fn_body fcall)) ->
+  forall base_env base_fname,
+    store_safe_synthetic_direct_call_ready_exact_body_call_route_reachable_exact_body_target_provider
+      base_env base_fname.
+Proof.
+  intros Hexact_body_target base_env base_fname env fname _Hreachable.
+  exact (Hexact_body_target env fname).
+Qed.
+
 Lemma store_safe_synthetic_direct_call_ready_exact_body_call_route_reachable_package_provider_of_at_all :
   (forall env fname,
     store_safe_synthetic_direct_call_ready_exact_body_call_route_package_at
@@ -2754,6 +2785,42 @@ Proof.
   exact Hsummary.
 Qed.
 
+Lemma fn_root_shadow_synthetic_direct_call_ready_summary_evidence_at_of_exact_body_call_route_package_at_local :
+  forall env fname,
+    (forall fdef fcall used used' fname_body args_body synthetic_body,
+      In fdef (env_fns env) ->
+      fn_name fdef = fname ->
+      alpha_rename_fn_def used fdef = (fcall, used') ->
+      direct_call_target_expr (fn_body fcall) =
+        Some (fname_body, args_body, synthetic_body) ->
+      direct_call_target_expr (fn_body fcall) =
+        Some (fname_body, args_body, fn_body fcall)) ->
+    store_safe_synthetic_direct_call_ready_exact_body_call_route_package_at
+      env fname ->
+  forall fdef fcall used used' fname_body args_body synthetic_body,
+    In fdef (env_fns env) ->
+    fn_name fdef = fname ->
+    alpha_rename_fn_def used fdef = (fcall, used') ->
+    direct_call_target_expr (fn_body fcall) =
+      Some (fname_body, args_body, synthetic_body) ->
+    fn_root_shadow_synthetic_direct_call_ready_summary_evidence_at
+      (global_env_with_local_bounds env (fn_bounds fcall)) fname_body.
+Proof.
+  intros env fname Hexact_body_target Hbody_package fdef fcall used used'
+    fname_body args_body synthetic_body Hin Hname Hrename Htarget.
+  pose proof
+    (Hexact_body_target fdef fcall used used' fname_body args_body
+      synthetic_body Hin Hname Hrename Htarget) as Htarget_exact.
+  pose proof
+    (direct_call_target_expr_same_is_call (fn_body fcall) fname_body
+      args_body Htarget_exact) as Hbody_exact.
+  destruct
+    (Hbody_package fdef fcall used used' fname_body args_body
+      Hin Hname Hrename) as [Hsummary _].
+  { rewrite <- Hbody_exact. exact Htarget_exact. }
+  exact Hsummary.
+Qed.
+
 Lemma store_safe_function_value_call_args_of_exact_body_call_route_package :
   (forall env fname fdef fcall used used' fname_body args_body synthetic_body,
     In fdef (env_fns env) ->
@@ -2814,6 +2881,42 @@ Proof.
   pose proof
     (Hexact_body_target env fname fdef fcall used used' fname_body
       args_body synthetic_body Hin Hname Hrename Htarget) as Htarget_exact.
+  pose proof
+    (direct_call_target_expr_same_is_call (fn_body fcall) fname_body
+      args_body Htarget_exact) as Hbody_exact.
+  destruct
+    (Hbody_package fdef fcall used used' fname_body args_body
+      Hin Hname Hrename) as [_ Hsafe].
+  { rewrite <- Hbody_exact. exact Htarget_exact. }
+  exact Hsafe.
+Qed.
+
+Lemma store_safe_function_value_call_args_of_exact_body_call_route_package_at_local :
+  forall env fname,
+    (forall fdef fcall used used' fname_body args_body synthetic_body,
+      In fdef (env_fns env) ->
+      fn_name fdef = fname ->
+      alpha_rename_fn_def used fdef = (fcall, used') ->
+      direct_call_target_expr (fn_body fcall) =
+        Some (fname_body, args_body, synthetic_body) ->
+      direct_call_target_expr (fn_body fcall) =
+        Some (fname_body, args_body, fn_body fcall)) ->
+    store_safe_synthetic_direct_call_ready_exact_body_call_route_package_at
+      env fname ->
+  forall fdef fcall used used' fname_body args_body synthetic_body,
+    In fdef (env_fns env) ->
+    fn_name fdef = fname ->
+    alpha_rename_fn_def used fdef = (fcall, used') ->
+    direct_call_target_expr (fn_body fcall) =
+      Some (fname_body, args_body, synthetic_body) ->
+    store_safe_function_value_call_args
+      (global_env_with_local_bounds env (fn_bounds fcall)) args_body.
+Proof.
+  intros env fname Hexact_body_target Hbody_package fdef fcall used used'
+    fname_body args_body synthetic_body Hin Hname Hrename Htarget.
+  pose proof
+    (Hexact_body_target fdef fcall used used' fname_body args_body
+      synthetic_body Hin Hname Hrename Htarget) as Htarget_exact.
   pose proof
     (direct_call_target_expr_same_is_call (fn_body fcall) fname_body
       args_body Htarget_exact) as Hbody_exact.
@@ -10253,6 +10356,302 @@ Proof.
 Qed.
 
 
+
+Theorem eval_preserves_typing_roots_synthetic_direct_call_ready_summary_at_prefix_call_height_statement_evidence_at_current_from_reachable_less_callbacks_and_exact_body_call_route_package_and_target_provider :
+  eval_preserves_typing_ready_prefix_mutual_statement ->
+  eval_preserves_typing_roots_ready_prefix_mutual_statement ->
+  eval_preserves_roots_ready_mutual_statement ->
+  eval_preserves_root_names_ready_mutual_statement ->
+  eval_preserves_root_keys_named_ready_mutual_statement ->
+  preservation_ready_expr_static_runtime_named_statement ->
+  forall base_env base_fname env s fname args s' v n_call,
+    store_safe_synthetic_direct_call_ready_exact_body_call_route_reachable
+      base_env base_fname env fname ->
+    store_safe_synthetic_direct_call_ready_exact_body_call_route_reachable_exact_body_target_provider
+      base_env base_fname ->
+    store_safe_synthetic_direct_call_ready_exact_body_call_route_reachable_package_provider
+      base_env base_fname ->
+    eval env s (ECall fname args) s' v ->
+    direct_call_eval_height env s (ECall fname args) s' v n_call ->
+    eval_preserves_typing_roots_synthetic_direct_call_ready_summary_at_prefix_call_height_statement_evidence_at_reachable_less_callback
+      base_env base_fname n_call ->
+    eval_preserves_frame_param_scope_synthetic_direct_call_ready_summary_at_prefix_call_height_statement_evidence_at_reachable_less_callback
+      base_env base_fname n_call ->
+    forall (Omega : outlives_ctx) (n : nat) R Σ T Σ' R' roots,
+      preservation_ready_args args ->
+      store_typed_prefix env s Σ ->
+      store_roots_within R s ->
+      store_no_shadow s ->
+      root_env_no_shadow R ->
+      root_env_store_roots_named R s ->
+      root_env_store_keys_named R s ->
+      typed_env_roots env Omega n R Σ (ECall fname args) T Σ' R' roots ->
+      fn_env_unique_by_name env ->
+      fn_root_shadow_synthetic_direct_call_ready_summary_evidence_at env fname ->
+      direct_call_callee_body_root_synthetic_direct_call_ready_evidence_at
+        env fname ->
+      store_typed_prefix env s' Σ' /\
+      value_has_type env s' v T /\
+      store_ref_targets_preserved env s s' /\
+      store_roots_within R' s' /\
+      value_roots_within roots v /\
+      store_no_shadow s' /\
+      root_env_no_shadow R'.
+Proof.
+  intros Htyping_prefix Hprefix_ready Hroots_ready Hroot_names Hroot_keys
+    Hstatic base_env base_fname env s fname args s' v n_call Hreachable
+    Htarget_provider Hprovider Heval_call Hheight_call Htyping_less
+    Hscope_less Omega n R Σ T Σ' R' roots Hready_args Hstore Hroots
+    Hshadow Hrn Hnamed Hkeys Htyped Hunique Hsummary_at Hevidence_at.
+  pose proof (Hprovider env fname Hreachable) as Hbody_package.
+  pose proof
+    (fun fdef fcall used used' fname_body args_body synthetic_body
+        Hin Hname Hrename Htarget =>
+      fn_root_shadow_synthetic_direct_call_ready_summary_evidence_at_of_exact_body_call_route_package_at_local
+        env fname (Htarget_provider env fname Hreachable) Hbody_package fdef fcall used used'
+        fname_body args_body synthetic_body Hin Hname Hrename Htarget)
+    as Hsummary_body_at_alpha.
+  pose proof
+    (fun fdef fcall used used' fname_body args_body
+        Hin Hname Hrename Htarget =>
+      direct_call_target_expr_same_is_call (fn_body fcall) fname_body args_body
+        ((Htarget_provider env fname Hreachable) fdef fcall used used' fname_body
+          args_body (ECall fname_body args_body) Hin Hname Hrename Htarget))
+    as Hbody_exact.
+  pose proof (preservation_ready_args_implies_provenance_ready_closure
+                args Hready_args) as Hprov_args.
+  dependent destruction Heval_call.
+  dependent destruction Htyped.
+  simpl in *.
+  repeat match goal with
+  | Hlookup : lookup_fn (fn_name ?f_typed) (env_fns env) =
+      Some ?f_runtime,
+    Hin0 : In ?f_typed (env_fns env) |- _ =>
+      pose proof (lookup_fn_unique_by_name env (fn_name f_typed)
+        f_runtime f_typed Hlookup Hin0 eq_refl Hunique) as Hsame;
+      subst f_runtime
+  | Hlookup : lookup_fn ?fname_call (env_fns env) = Some ?f_runtime,
+    Hin0 : In ?f_typed (env_fns env),
+    Hname : fn_name ?f_typed = ?fname_call |- _ =>
+      pose proof (lookup_fn_unique_by_name env fname_call f_runtime f_typed
+        Hlookup Hin0 Hname Hunique) as Hsame;
+      subst f_typed
+  | Hlookup : lookup_fn ?fname_call (env_fns env) = Some ?f_runtime,
+    Hin0 : In ?f_typed (env_fns env),
+    Hname : ?fname_call = fn_name ?f_typed |- _ =>
+      pose proof (lookup_fn_unique_by_name env fname_call f_runtime f_typed
+        Hlookup Hin0 (eq_sym Hname) Hunique) as Hsame;
+      subst f_typed
+  end.
+  destruct (proj1 (proj2 Hroots_ready)
+              env s args s_args vs H1 Omega n R Σ
+              (apply_lt_params σ (fn_params fdef0)) Σ' R'
+              arg_roots Hprov_args Hroots Hshadow Hrn H7)
+    as [Hroots_args [_ [Hshadow_args Hrn_args]]].
+  destruct (proj1 (proj2 Htyping_prefix)
+              env s args s_args vs H1 Omega n Σ
+              (apply_lt_params σ (fn_params fdef0)) Σ'
+              Hready_args Hstore
+              (typed_args_roots_structural env Omega n R Σ args
+                (apply_lt_params σ (fn_params fdef0)) Σ' R'
+                arg_roots H7))
+    as [_ [Hargs_subst _]].
+  pose proof (alpha_rename_fn_def_shape (store_names s_args)
+                fdef0 fcall used' H2) as Hshape.
+  destruct Hshape as [_ [_ Hparams_alpha]].
+  assert (Hargs_unsubst_fdef :
+    eval_args_values_have_types env Omega s_args vs (fn_params fdef0)).
+  { eapply eval_args_values_have_types_apply_lt_params_inv.
+    exact Hargs_subst. }
+  assert (Hargs_fcall :
+    eval_args_values_have_types env Omega s_args vs (fn_params fcall)).
+  { eapply eval_args_values_have_types_params_alpha.
+    - exact Hparams_alpha.
+    - exact Hargs_unsubst_fdef. }
+  assert (Hnodup :
+    NoDup (ctx_names (params_ctx (fn_params fcall)))).
+  { eapply alpha_rename_fn_def_params_nodup_ctx_names. exact H2. }
+  assert (Hfresh : params_fresh_in_store (fn_params fcall) s_args).
+  { eapply alpha_rename_fn_def_params_fresh_in_store. exact H2. }
+  destruct (eval_args_bind_params_call_param_root_env_ready
+              env s args s_args vs Omega n R Σ
+              (apply_lt_params σ (fn_params fdef0)) Σ' R' arg_roots
+              (fn_params fcall) H1 Hprov_args H7
+              Hroots Hshadow Hrn Hnodup Hfresh Hargs_fcall)
+    as [Hroots_bind [Hshadow_bind [Hrn_bind _Hcover_bind]]].
+  destruct
+    (eval_args_preserves_root_names_keys_preservation_ready_runtime_with_static_expr
+      Hstatic env s args s_args vs Omega n R Σ
+      (apply_lt_params σ (fn_params fdef0)) Σ' R' arg_roots
+      H1 Hready_args Hrn Hroots Hnamed Hkeys H7)
+    as [Hnamed_args [Harg_roots_named Hkeys_args]].
+  assert (Hnamed_bind :
+    root_env_store_roots_named
+      (call_param_root_env (fn_params fcall) arg_roots R')
+      (bind_params (fn_params fcall) vs s_args)).
+  { eapply root_env_store_roots_named_call_param_bind_params;
+      eassumption. }
+  assert (Hkeys_bind :
+    root_env_store_keys_named
+      (call_param_root_env (fn_params fcall) arg_roots R')
+      (bind_params (fn_params fcall) vs s_args)).
+  { eapply root_env_store_keys_named_call_param_bind_params;
+      eassumption. }
+  assert (Hstore_bind_env :
+    store_typed_prefix env (bind_params (fn_params fcall) vs s_args)
+      (sctx_of_ctx (params_ctx (fn_params fcall)))).
+  { eapply bind_params_store_typed_prefix; eassumption. }
+  assert (Hstore_bind_body_env :
+    store_typed_prefix (global_env_with_local_bounds env (fn_bounds fcall))
+      (bind_params (fn_params fcall) vs s_args)
+      (sctx_of_ctx (params_ctx (fn_params fcall)))).
+  { eapply direct_call_store_typed_prefix_global_env_with_local_bounds.
+    exact Hstore_bind_env. }
+  pose proof
+    (callee_body_root_shadow_synthetic_direct_call_ready_result_subset_from_summary_at_prefix_store
+      Hprefix_ready env Omega n R Σ Σ' R' arg_roots
+      (fn_name fdef0) args fdef0 fcall σ s s_args vs used' Hunique
+      Hsummary_at H3 eq_refl H0 H7 H1 Hprov_args Hstore Hroots Hshadow Hrn
+      Hnamed Hkeys Hnamed_args Harg_roots_named Hkeys_args H2)
+    as Hbody_result_subset.
+  pose proof
+    (eval_synthetic_direct_call_body_scope_callback_from_result_subset_prefix_store_body_callback_with_height
+      Hprefix_ready env Omega n R Σ Σ' R' arg_roots
+      (fn_name fdef0) args fdef0 fcall σ s s_args s_body vs ret used'
+      Hbody_result_subset H3 eq_refl H0 H7 H1 Hready_args Hprov_args Hstore
+      Hroots Hshadow Hrn H2 Heval_call
+      (fun fname_body args_body T_body Gamma_out R_body roots_body n_body_call
+          Htarget_body Hready_args_body Htyped_body Heval_synthetic_body_env
+          Hheight_body_env Hroots_bind' Hshadow_bind' Hrn_bind'
+          Hcover_params Hframe_start Hframe_fresh_start Hparam_start =>
+        let Hbody_eq :=
+          Hbody_exact fdef0 fcall (store_names s_args) used'
+            fname_body args_body H3 eq_refl H2 Htarget_body in
+        match
+          direct_call_eval_height_ecall_body_lt_of_eval_call env s s_args
+            s_body (fn_name fdef0) args fdef0 fcall vs ret used' n_call
+            H H0 H1 H2 Heval_call Hheight_call
+        with
+        | ex_intro _ n_body_call0 (conj Hheight_body Hlt_body) =>
+            let Hheight_body' :=
+              eq_rect _
+                (fun body =>
+                  direct_call_eval_height env
+                    (bind_params (fn_params fcall) vs s_args) body s_body ret
+                    n_body_call0)
+                Hheight_body _ Hbody_eq in
+            let Hheight_body_global :=
+              direct_call_eval_height_global_env_with_local_bounds env
+                (fn_bounds fcall)
+                (bind_params (fn_params fcall) vs s_args)
+                (ECall fname_body args_body) s_body ret n_body_call0
+                Hheight_body' in
+            let Hsummary_body :=
+              Hsummary_body_at_alpha fdef0 fcall (store_names s_args) used'
+                fname_body args_body (ECall fname_body args_body) H3 eq_refl
+                H2 Htarget_body in
+            let Hunique_body :
+              fn_env_unique_by_name
+                (global_env_with_local_bounds env (fn_bounds fcall)) :=
+              Hunique in
+            let Hevidence_body :=
+              direct_call_callee_body_root_synthetic_direct_call_ready_evidence_at_of_shadow_summary_at
+                Hroot_names Hroot_keys
+                (global_env_with_local_bounds env (fn_bounds fcall))
+                fname_body Hsummary_body Hunique_body in
+            let Hreachable_body :=
+              store_safe_synthetic_direct_call_ready_exact_body_call_route_reachable_body_call_step
+                base_env base_fname env (fn_name fdef0) fdef0 fcall (store_names s_args)
+                used' fname_body args_body Hreachable H3 eq_refl H2
+                Htarget_body in
+            match
+              Hscope_less n_body_call0 Hlt_body
+                (global_env_with_local_bounds env (fn_bounds fcall))
+                fname_body Hreachable_body
+                (bind_params (fn_params fcall) vs s_args) args_body
+                s_body ret Heval_synthetic_body_env Hheight_body_global
+                (fn_outlives fcall) (fn_lifetimes fcall)
+                (call_param_root_env (fn_params fcall) arg_roots R')
+                (sctx_of_ctx (params_ctx (fn_params fcall))) T_body
+                (sctx_of_ctx Gamma_out) R_body roots_body (fn_params fcall)
+                s_args Hready_args_body Hstore_bind_body_env Hnamed_bind
+                Hkeys_bind Htyped_body Hunique_body Hsummary_body Hevidence_body
+                Hcover_params Hroots_bind' Hshadow_bind' Hrn_bind'
+                Hframe_start Hframe_fresh_start Hparam_start
+            with
+            | conj Hframe_body (ex_intro _ frame_final Hparam_body) =>
+                ex_intro _ frame_final (conj Hframe_body Hparam_body)
+            end
+        end)) as Hscopes.
+  destruct
+    (eval_synthetic_direct_call_body_cleanup_prefix_from_result_subset_summary_at_call_statement_body_call_callback_prefix_store
+      Hprefix_ready Hroots_ready Hroot_names Hroot_keys
+      env Omega n R Σ Σ' R' arg_roots (fn_name fdef0) args fdef0 fcall
+      σ s s_args s_body vs ret used' Hbody_result_subset
+      (fun fname_body args_body synthetic_body Htarget_body =>
+        Hsummary_body_at_alpha fdef0 fcall (store_names s_args) used'
+          fname_body args_body synthetic_body H3 eq_refl H2 Htarget_body)
+      (fun fname_body args_body T_body Gamma_out R_body roots_body
+          Htarget_body Hready_args_body Htyped_body Hunique_body_env
+          Hsummary_body_at' Hready_evidence_at Hstore_bind_body_env'
+          Hroots_bind' Hshadow_bind' Hrn_bind' Hnamed_bind' Hkeys_bind'
+          Heval_synthetic_body_env =>
+        let Hbody_eq :=
+          Hbody_exact fdef0 fcall (store_names s_args) used'
+            fname_body args_body H3 eq_refl H2 Htarget_body in
+        match
+          direct_call_eval_height_ecall_body_lt_of_eval_call env s s_args
+            s_body (fn_name fdef0) args fdef0 fcall vs ret used' n_call
+            H H0 H1 H2 Heval_call Hheight_call
+        with
+        | ex_intro _ n_body_call (conj Hheight_body Hlt_body) =>
+            let Hheight_body' :=
+              eq_rect _
+                (fun body =>
+                  direct_call_eval_height env
+                    (bind_params (fn_params fcall) vs s_args) body s_body ret
+                    n_body_call)
+                Hheight_body _ Hbody_eq in
+            let Hreachable_body :=
+              store_safe_synthetic_direct_call_ready_exact_body_call_route_reachable_body_call_step
+                base_env base_fname env (fn_name fdef0) fdef0 fcall (store_names s_args)
+                used' fname_body args_body Hreachable H3 eq_refl H2
+                Htarget_body in
+            Htyping_less n_body_call Hlt_body
+              (global_env_with_local_bounds env (fn_bounds fcall))
+              fname_body Hreachable_body
+              (bind_params (fn_params fcall) vs s_args) args_body
+              s_body ret Heval_synthetic_body_env
+              (direct_call_eval_height_global_env_with_local_bounds env
+                (fn_bounds fcall)
+                (bind_params (fn_params fcall) vs s_args)
+                (ECall fname_body args_body) s_body ret n_body_call
+                Hheight_body')
+              (fn_outlives fcall) (fn_lifetimes fcall)
+              (call_param_root_env (fn_params fcall) arg_roots R')
+              (sctx_of_ctx (params_ctx (fn_params fcall))) T_body
+              (sctx_of_ctx Gamma_out) R_body roots_body Hready_args_body
+              Hstore_bind_body_env' Hroots_bind' Hshadow_bind' Hrn_bind'
+              Hnamed_bind' Hkeys_bind' Htyped_body Hunique_body_env
+              Hsummary_body_at' Hready_evidence_at
+        end)
+      Hunique H3 eq_refl H0 H7 H1 Hready_args Hprov_args Hstore Hroots
+      Hshadow Hrn Hnamed Hkeys H2 Hstore_bind_body_env Hroots_bind
+      Hshadow_bind Hrn_bind Hnamed_bind Hkeys_bind Heval_call Hscopes)
+    as (_fname_body & _args_body & _synthetic_body & _T_body & _Gamma_out &
+        _R_body & roots_body & _frame_final & _locals & _Htarget &
+        _Hsynthetic & _Hready_body & _Htyped_body & _Hcompat_body &
+        _Hexclude_roots & _Hexclude_env & Hresult_subset & _Heval_synthetic &
+        _Hstore_args & Hstore_final & _Hstore_prefix & _Hroots_body &
+        _Hshadow_body & _Hrn_body & Hv_final & Hpres_final & _Hremoved &
+        _Hret_exclude & _Hstore_exclude & Hremoved_exact & Hret_roots).
+  repeat split; try assumption.
+  - rewrite Hremoved_exact. exact Hroots_args.
+  - eapply direct_call_value_roots_within_store_subset; eassumption.
+  - rewrite Hremoved_exact. exact Hshadow_args.
+Qed.
+
+
 Theorem eval_preserves_typing_roots_synthetic_direct_call_ready_ecall_cleanup_bridge_with_alpha_evidence_at_decreasing_body_call_callback_prefix_store_final_roots_core_exact_body :
   eval_preserves_frame_param_scope_synthetic_direct_call_ready_statement ->
   eval_preserves_typing_ready_prefix_mutual_statement ->
@@ -12544,11 +12943,12 @@ Proof.
   intros Htyping_prefix Hprefix_ready Hroots_ready Hroot_names Hroot_keys
     Hstatic Hframe_ready Hparam_ready Hexact_body_target.
   intros base_env base_fname env s fname args s' v n_call0 Hreachable
-    Hprovider Heval_call Hheight_call Htyping_less Hscope_less Omega n R Σ T
-    Σ' R' roots ps frame Hready_args Hstore Hnamed Hkeys
-    Htyped Hunique Hsummary_at Hevidence_at Hcover Hroots Hshadow Hrn Hframe
-    Hfresh Hparam.
-  pose proof (Hprovider env fname Hreachable) as Hbody_package.
+    Hreachable_package_provider Heval_call Hheight_call Htyping_less
+    Hscope_less Omega n R Σ T Σ' R' roots ps frame Hready_args Hstore
+    Hnamed Hkeys Htyped Hunique Hsummary_at Hevidence_at Hcover Hroots
+    Hshadow Hrn Hframe Hfresh Hparam.
+  pose proof (Hreachable_package_provider env fname Hreachable)
+    as Hbody_package.
   pose proof (preservation_ready_args_implies_provenance_ready_closure
                 args Hready_args) as Hprov_args.
   dependent destruction Heval_call.
@@ -12748,6 +13148,314 @@ Proof.
           Heval_synthetic_body_env =>
         let Htarget_exact :=
           Hexact_body_target env (fn_name fdef0) fdef0 fcall
+            (store_names s_args) used' fname_body args_body
+            (ECall fname_body args_body) H3 eq_refl H2 Htarget_body in
+        let Hbody_eq :=
+          direct_call_target_expr_same_is_call (fn_body fcall) fname_body
+            args_body Htarget_exact in
+        match
+          direct_call_eval_height_ecall_body_lt_of_eval_call env s s_args
+            s_body (fn_name fdef0) args fdef0 fcall vs ret used' n_call0
+            H H5 H1 H2 Heval_call Hheight_call
+        with
+        | ex_intro _ n_body_call0 (conj Hheight_body Hlt_body) =>
+            let Hheight_body' :=
+              eq_rect _
+                (fun body =>
+                  direct_call_eval_height env
+                    (bind_params (fn_params fcall) vs s_args) body s_body ret
+                    n_body_call0)
+                Hheight_body _ Hbody_eq in
+            let Hheight_body_global :=
+              direct_call_eval_height_global_env_with_local_bounds env
+                (fn_bounds fcall)
+                (bind_params (fn_params fcall) vs s_args)
+                (ECall fname_body args_body) s_body ret n_body_call0
+                Hheight_body' in
+            let Hreachable_body :=
+              store_safe_synthetic_direct_call_ready_exact_body_call_route_reachable_body_call_step
+                base_env base_fname env (fn_name fdef0) fdef0 fcall (store_names s_args)
+                used' fname_body args_body Hreachable H3 eq_refl H2
+                Htarget_body in
+            Htyping_less n_body_call0 Hlt_body
+              (global_env_with_local_bounds env (fn_bounds fcall))
+              fname_body Hreachable_body
+              (bind_params (fn_params fcall) vs s_args) args_body
+              s_body ret Heval_synthetic_body_env Hheight_body_global
+              (fn_outlives fcall) (fn_lifetimes fcall)
+              (call_param_root_env (fn_params fcall) arg_roots R')
+              (sctx_of_ctx (params_ctx (fn_params fcall))) T_body
+              (sctx_of_ctx Gamma_out) R_body roots_body Hready_args_body
+              Hstore_bind_body_env' Hroots_bind' Hshadow_bind' Hrn_bind'
+              Hnamed_bind' Hkeys_bind' Htyped_body Hunique_body_env
+              Hsummary_body_at' Hready_evidence_at
+        end)
+      Hunique H3 eq_refl H5 H7 H1 Hready_args Hprov_args Hstore Hroots
+      Hshadow Hrn Hnamed Hkeys H2 Hstore_bind_body_env Hroots_bind
+      Hshadow_bind Hrn_bind Hnamed_bind Hkeys_bind Heval_call Hscopes)
+    as (_fname_body & _args_body & _synthetic_body & _T_body & _Gamma_out &
+        _R_body & _roots_body & _frame_final & _locals & _Htarget &
+        _Hsynthetic & _Hready_body & _Htyped_body & _Hcompat_body &
+        _Hexclude_roots & _Hexclude_env & _Hresult_subset & _Heval_synthetic &
+        _Hstore_args & _Hstore_final & _Hstore_prefix & _Hroots_body &
+        _Hshadow_body & _Hrn_body & _Hv_final & _Hpres_final & _Hremoved &
+        _Hret_exclude & _Hstore_exclude & Hremoved_exact & _Hret_roots).
+  split.
+  - rewrite Hremoved_exact. exact Hframe_args.
+  - exists frame_args. rewrite Hremoved_exact. exact Hparam_args.
+Qed.
+
+
+Theorem eval_preserves_frame_param_scope_synthetic_direct_call_ready_summary_at_prefix_call_height_statement_evidence_at_current_from_reachable_less_callbacks_and_exact_body_call_route_package_and_target_provider :
+  eval_preserves_typing_ready_prefix_mutual_statement ->
+  eval_preserves_typing_roots_ready_prefix_mutual_statement ->
+  eval_preserves_roots_ready_mutual_statement ->
+  eval_preserves_root_names_ready_mutual_statement ->
+  eval_preserves_root_keys_named_ready_mutual_statement ->
+  preservation_ready_expr_static_runtime_named_statement ->
+  eval_preserves_frame_scope_roots_ready_mutual_statement ->
+  eval_preserves_param_scope_roots_ready_mutual_statement ->
+  forall base_env base_fname env s fname args s' v n_call,
+    store_safe_synthetic_direct_call_ready_exact_body_call_route_reachable
+      base_env base_fname env fname ->
+    store_safe_synthetic_direct_call_ready_exact_body_call_route_reachable_exact_body_target_provider
+      base_env base_fname ->
+    store_safe_synthetic_direct_call_ready_exact_body_call_route_reachable_package_provider
+      base_env base_fname ->
+    eval env s (ECall fname args) s' v ->
+    direct_call_eval_height env s (ECall fname args) s' v n_call ->
+    eval_preserves_typing_roots_synthetic_direct_call_ready_summary_at_prefix_call_height_statement_evidence_at_reachable_less_callback
+      base_env base_fname n_call ->
+    eval_preserves_frame_param_scope_synthetic_direct_call_ready_summary_at_prefix_call_height_statement_evidence_at_reachable_less_callback
+      base_env base_fname n_call ->
+    forall (Omega : outlives_ctx) (n : nat) R Σ T Σ' R' roots
+        ps frame,
+      preservation_ready_args args ->
+      store_typed_prefix env s Σ ->
+      root_env_store_roots_named R s ->
+      root_env_store_keys_named R s ->
+      typed_env_roots env Omega n R Σ (ECall fname args) T Σ' R' roots ->
+      fn_env_unique_by_name env ->
+      fn_root_shadow_synthetic_direct_call_ready_summary_evidence_at env fname ->
+      direct_call_callee_body_root_synthetic_direct_call_ready_evidence_at
+        env fname ->
+      root_env_covers_params ps R ->
+      store_roots_within R s ->
+      store_no_shadow s ->
+      root_env_no_shadow R ->
+      store_frame_scope ps Σ s frame ->
+      store_frame_static_fresh Σ frame ->
+      store_param_scope ps s frame ->
+      store_frame_scope ps Σ' s' frame /\
+      exists frame', store_param_scope ps s' frame'.
+Proof.
+  intros Htyping_prefix Hprefix_ready Hroots_ready Hroot_names Hroot_keys
+    Hstatic Hframe_ready Hparam_ready base_env base_fname env s fname args s' v
+    n_call0 Hreachable Htarget_provider Hprovider Heval_call Hheight_call
+    Htyping_less Hscope_less Omega n R Σ T Σ' R' roots ps frame
+    Hready_args Hstore Hnamed Hkeys Htyped Hunique Hsummary_at Hevidence_at
+    Hcover Hroots Hshadow Hrn Hframe Hfresh Hparam.
+  pose proof (Hprovider env fname Hreachable) as Hbody_package.
+  pose proof (preservation_ready_args_implies_provenance_ready_closure
+                args Hready_args) as Hprov_args.
+  dependent destruction Heval_call.
+  dependent destruction Htyped.
+  simpl in *.
+  repeat match goal with
+  | Hlookup : lookup_fn (fn_name ?f_typed) (env_fns env) =
+      Some ?f_runtime,
+    Hin0 : In ?f_typed (env_fns env) |- _ =>
+      pose proof (lookup_fn_unique_by_name env (fn_name f_typed)
+        f_runtime f_typed Hlookup Hin0 eq_refl Hunique) as Hsame;
+      subst f_runtime
+  | Hlookup : lookup_fn ?fname_call (env_fns env) = Some ?f_runtime,
+    Hin0 : In ?f_typed (env_fns env),
+    Hname : fn_name ?f_typed = ?fname_call |- _ =>
+      pose proof (lookup_fn_unique_by_name env fname_call f_runtime f_typed
+        Hlookup Hin0 Hname Hunique) as Hsame;
+      subst f_typed
+  | Hlookup : lookup_fn ?fname_call (env_fns env) = Some ?f_runtime,
+    Hin0 : In ?f_typed (env_fns env),
+    Hname : ?fname_call = fn_name ?f_typed |- _ =>
+      pose proof (lookup_fn_unique_by_name env fname_call f_runtime f_typed
+        Hlookup Hin0 (eq_sym Hname) Hunique) as Hsame;
+      subst f_typed
+  end.
+  destruct
+    (eval_args_preserves_frame_param_scope_roots_ready
+      Hframe_ready Hparam_ready env s args s_args vs Omega n R Σ
+      (apply_lt_params σ (fn_params fdef0)) Σ' R' arg_roots ps frame H1
+      Hprov_args H7 Hcover Hroots Hshadow Hrn Hframe Hfresh Hparam)
+    as [Hframe_args [frame_args Hparam_args]].
+  destruct (proj1 (proj2 Hroots_ready)
+              env s args s_args vs H1 Omega n R Σ
+              (apply_lt_params σ (fn_params fdef0)) Σ' R'
+              arg_roots Hprov_args Hroots Hshadow Hrn H7)
+    as [_ [_ [_ Hrn_args]]].
+  destruct (proj1 (proj2 Htyping_prefix)
+              env s args s_args vs H1 Omega n Σ
+              (apply_lt_params σ (fn_params fdef0)) Σ'
+              Hready_args Hstore
+              (typed_args_roots_structural env Omega n R Σ args
+                (apply_lt_params σ (fn_params fdef0)) Σ' R'
+                arg_roots H7))
+    as [_ [Hargs_subst _]].
+  pose proof (alpha_rename_fn_def_shape (store_names s_args)
+                fdef0 fcall used' H2) as Hshape.
+  destruct Hshape as [_ [_ Hparams_alpha]].
+  assert (Hargs_unsubst_fdef :
+    eval_args_values_have_types env Omega s_args vs (fn_params fdef0)).
+  { eapply eval_args_values_have_types_apply_lt_params_inv.
+    exact Hargs_subst. }
+  assert (Hargs_fcall :
+    eval_args_values_have_types env Omega s_args vs (fn_params fcall)).
+  { eapply eval_args_values_have_types_params_alpha.
+    - exact Hparams_alpha.
+    - exact Hargs_unsubst_fdef. }
+  assert (Hnodup :
+    NoDup (ctx_names (params_ctx (fn_params fcall)))).
+  { eapply alpha_rename_fn_def_params_nodup_ctx_names. exact H2. }
+  assert (Hfresh_params : params_fresh_in_store (fn_params fcall) s_args).
+  { eapply alpha_rename_fn_def_params_fresh_in_store. exact H2. }
+  destruct (eval_args_bind_params_call_param_root_env_ready
+              env s args s_args vs Omega n R Σ
+              (apply_lt_params σ (fn_params fdef0)) Σ' R' arg_roots
+              (fn_params fcall) H1 Hprov_args H7
+              Hroots Hshadow Hrn Hnodup Hfresh_params Hargs_fcall)
+    as [Hroots_bind [Hshadow_bind [Hrn_bind _Hcover_bind]]].
+  destruct
+    (eval_args_preserves_root_names_keys_preservation_ready_runtime_with_static_expr
+      Hstatic env s args s_args vs Omega n R Σ
+      (apply_lt_params σ (fn_params fdef0)) Σ' R' arg_roots H1
+      Hready_args Hrn Hroots Hnamed Hkeys H7)
+    as [Hnamed_args [Harg_roots_named Hkeys_args]].
+  assert (Hnamed_bind :
+    root_env_store_roots_named
+      (call_param_root_env (fn_params fcall) arg_roots R')
+      (bind_params (fn_params fcall) vs s_args)).
+  { eapply root_env_store_roots_named_call_param_bind_params
+      with (env := env) (Ω := Omega).
+    - exact Hargs_fcall.
+    - exact Harg_roots_named.
+    - exact Hrn_args.
+    - exact Hnamed_args. }
+  assert (Hkeys_bind :
+    root_env_store_keys_named
+      (call_param_root_env (fn_params fcall) arg_roots R')
+      (bind_params (fn_params fcall) vs s_args)).
+  { eapply root_env_store_keys_named_call_param_bind_params
+      with (env := env) (Ω := Omega).
+    - exact Hargs_fcall.
+    - exact Hkeys_args. }
+  assert (Hstore_bind_env :
+    store_typed_prefix env (bind_params (fn_params fcall) vs s_args)
+      (sctx_of_ctx (params_ctx (fn_params fcall)))).
+  { eapply bind_params_store_typed_prefix; eassumption. }
+  assert (Hstore_bind_body_env :
+    store_typed_prefix (global_env_with_local_bounds env (fn_bounds fcall))
+      (bind_params (fn_params fcall) vs s_args)
+      (sctx_of_ctx (params_ctx (fn_params fcall)))).
+  { eapply direct_call_store_typed_prefix_global_env_with_local_bounds.
+    exact Hstore_bind_env. }
+  pose proof
+    (callee_body_root_shadow_synthetic_direct_call_ready_result_subset_from_summary_at_prefix_store
+      Hprefix_ready env Omega n R Σ Σ' R' arg_roots
+      (fn_name fdef0) args fdef0 fcall σ s s_args vs used' Hunique
+      Hsummary_at H3 eq_refl H5 H7 H1 Hprov_args Hstore Hroots Hshadow Hrn
+      Hnamed Hkeys Hnamed_args Harg_roots_named Hkeys_args H2)
+    as Hbody_result_subset.
+  pose proof
+    (eval_synthetic_direct_call_body_scope_callback_from_result_subset_prefix_store_body_callback_with_height
+      Hprefix_ready env Omega n R Σ Σ' R' arg_roots
+      (fn_name fdef0) args fdef0 fcall σ s s_args s_body vs ret used'
+      Hbody_result_subset H3 eq_refl H5 H7 H1 Hready_args Hprov_args Hstore
+      Hroots Hshadow Hrn H2 Heval_call
+      (fun fname_body args_body T_body Gamma_out R_body roots_body n_body_call
+          Htarget_body Hready_args_body Htyped_body Heval_synthetic_body_env
+          Hheight_body_env Hroots_bind' Hshadow_bind' Hrn_bind'
+          Hcover_params Hframe_start Hframe_fresh_start Hparam_start =>
+        let Htarget_exact :=
+          (Htarget_provider env (fn_name fdef0) Hreachable) fdef0 fcall
+            (store_names s_args) used' fname_body args_body
+            (ECall fname_body args_body) H3 eq_refl H2 Htarget_body in
+        let Hbody_eq :=
+          direct_call_target_expr_same_is_call (fn_body fcall) fname_body
+            args_body Htarget_exact in
+        match
+          direct_call_eval_height_ecall_body_lt_of_eval_call env s s_args
+            s_body (fn_name fdef0) args fdef0 fcall vs ret used' n_call0
+            H H5 H1 H2 Heval_call Hheight_call
+        with
+        | ex_intro _ n_body_call0 (conj Hheight_body Hlt_body) =>
+            let Hheight_body' :=
+              eq_rect _
+                (fun body =>
+                  direct_call_eval_height env
+                    (bind_params (fn_params fcall) vs s_args) body s_body ret
+                    n_body_call0)
+                Hheight_body _ Hbody_eq in
+            let Hheight_body_global :=
+              direct_call_eval_height_global_env_with_local_bounds env
+                (fn_bounds fcall)
+                (bind_params (fn_params fcall) vs s_args)
+                (ECall fname_body args_body) s_body ret n_body_call0
+                Hheight_body' in
+            let Hsummary_body :=
+              fn_root_shadow_synthetic_direct_call_ready_summary_evidence_at_of_exact_body_call_route_package_at_local
+                env (fn_name fdef0) (Htarget_provider env (fn_name fdef0) Hreachable) Hbody_package fdef0
+                fcall (store_names s_args) used' fname_body args_body
+                (ECall fname_body args_body) H3 eq_refl H2 Htarget_body in
+            let Hunique_body :
+              fn_env_unique_by_name
+                (global_env_with_local_bounds env (fn_bounds fcall)) :=
+              Hunique in
+            let Hevidence_body :=
+              direct_call_callee_body_root_synthetic_direct_call_ready_evidence_at_of_shadow_summary_at
+                Hroot_names Hroot_keys
+                (global_env_with_local_bounds env (fn_bounds fcall))
+                fname_body Hsummary_body Hunique_body in
+            let Hreachable_body :=
+              store_safe_synthetic_direct_call_ready_exact_body_call_route_reachable_body_call_step
+                base_env base_fname env (fn_name fdef0) fdef0 fcall (store_names s_args)
+                used' fname_body args_body Hreachable H3 eq_refl H2
+                Htarget_body in
+            match
+              Hscope_less n_body_call0 Hlt_body
+                (global_env_with_local_bounds env (fn_bounds fcall))
+                fname_body Hreachable_body
+                (bind_params (fn_params fcall) vs s_args) args_body
+                s_body ret Heval_synthetic_body_env Hheight_body_global
+                (fn_outlives fcall) (fn_lifetimes fcall)
+                (call_param_root_env (fn_params fcall) arg_roots R')
+                (sctx_of_ctx (params_ctx (fn_params fcall))) T_body
+                (sctx_of_ctx Gamma_out) R_body roots_body (fn_params fcall)
+                s_args Hready_args_body Hstore_bind_body_env Hnamed_bind
+                Hkeys_bind Htyped_body Hunique_body Hsummary_body Hevidence_body
+                Hcover_params Hroots_bind' Hshadow_bind' Hrn_bind'
+                Hframe_start Hframe_fresh_start Hparam_start
+            with
+            | conj Hframe_body (ex_intro _ frame_final Hparam_body) =>
+                ex_intro _ frame_final (conj Hframe_body Hparam_body)
+            end
+        end)) as Hscopes.
+  destruct
+    (eval_synthetic_direct_call_body_cleanup_prefix_from_result_subset_summary_at_call_statement_body_call_callback_prefix_store
+      Hprefix_ready Hroots_ready Hroot_names Hroot_keys env Omega n R Σ
+      Σ' R' arg_roots (fn_name fdef0) args fdef0 fcall σ s s_args
+      s_body vs ret used' Hbody_result_subset
+      (fun fname_body args_body synthetic_body Htarget_body =>
+        fn_root_shadow_synthetic_direct_call_ready_summary_evidence_at_of_exact_body_call_route_package_at_local
+          env (fn_name fdef0) (Htarget_provider env (fn_name fdef0) Hreachable)
+          Hbody_package fdef0 fcall
+          (store_names s_args) used' fname_body args_body synthetic_body H3
+          eq_refl H2 Htarget_body)
+      (fun fname_body args_body T_body Gamma_out R_body roots_body
+          Htarget_body Hready_args_body Htyped_body Hunique_body_env
+          Hsummary_body_at' Hready_evidence_at Hstore_bind_body_env'
+          Hroots_bind' Hshadow_bind' Hrn_bind' Hnamed_bind' Hkeys_bind'
+          Heval_synthetic_body_env =>
+        let Htarget_exact :=
+          (Htarget_provider env (fn_name fdef0) Hreachable) fdef0 fcall
             (store_names s_args) used' fname_body args_body
             (ECall fname_body args_body) H3 eq_refl H2 Htarget_body in
         let Hbody_eq :=
@@ -13114,6 +13822,201 @@ Proof.
       Hfresh Hparam).
 Qed.
 
+Theorem eval_preserves_typing_roots_and_frame_param_scope_synthetic_direct_call_ready_summary_at_prefix_call_height_statement_evidence_at_of_reachable_exact_body_call_route_package_and_target_provider :
+  eval_preserves_typing_ready_prefix_mutual_statement ->
+  eval_preserves_typing_roots_ready_prefix_mutual_statement ->
+  eval_preserves_roots_ready_mutual_statement ->
+  eval_preserves_root_names_ready_mutual_statement ->
+  eval_preserves_root_keys_named_ready_mutual_statement ->
+  preservation_ready_expr_static_runtime_named_statement ->
+  eval_preserves_frame_scope_roots_ready_mutual_statement ->
+  eval_preserves_param_scope_roots_ready_mutual_statement ->
+  forall base_env base_fname,
+    store_safe_synthetic_direct_call_ready_exact_body_call_route_reachable_exact_body_target_provider
+      base_env base_fname ->
+    store_safe_synthetic_direct_call_ready_exact_body_call_route_reachable_package_provider
+      base_env base_fname ->
+    (forall env fname,
+      store_safe_synthetic_direct_call_ready_exact_body_call_route_reachable
+        base_env base_fname env fname ->
+      forall s args s' v n_call,
+        eval env s (ECall fname args) s' v ->
+        direct_call_eval_height env s (ECall fname args) s' v n_call ->
+        forall (Omega : outlives_ctx) (n : nat) R Σ T Σ' R' roots,
+          preservation_ready_args args ->
+          store_typed_prefix env s Σ ->
+          store_roots_within R s ->
+          store_no_shadow s ->
+          root_env_no_shadow R ->
+          root_env_store_roots_named R s ->
+          root_env_store_keys_named R s ->
+          typed_env_roots env Omega n R Σ (ECall fname args) T Σ' R'
+            roots ->
+          fn_env_unique_by_name env ->
+          fn_root_shadow_synthetic_direct_call_ready_summary_evidence_at env
+            fname ->
+          direct_call_callee_body_root_synthetic_direct_call_ready_evidence_at
+            env fname ->
+          store_typed_prefix env s' Σ' /\
+          value_has_type env s' v T /\
+          store_ref_targets_preserved env s s' /\
+          store_roots_within R' s' /\
+          value_roots_within roots v /\
+          store_no_shadow s' /\
+          root_env_no_shadow R') /\
+    (forall env fname,
+      store_safe_synthetic_direct_call_ready_exact_body_call_route_reachable
+        base_env base_fname env fname ->
+      forall s args s' v n_call,
+        eval env s (ECall fname args) s' v ->
+        direct_call_eval_height env s (ECall fname args) s' v n_call ->
+        forall (Omega : outlives_ctx) (n : nat) R Σ T Σ' R' roots
+            ps frame,
+          preservation_ready_args args ->
+          store_typed_prefix env s Σ ->
+          root_env_store_roots_named R s ->
+          root_env_store_keys_named R s ->
+          typed_env_roots env Omega n R Σ (ECall fname args) T Σ' R'
+            roots ->
+          fn_env_unique_by_name env ->
+          fn_root_shadow_synthetic_direct_call_ready_summary_evidence_at env
+            fname ->
+          direct_call_callee_body_root_synthetic_direct_call_ready_evidence_at
+            env fname ->
+          root_env_covers_params ps R ->
+          store_roots_within R s ->
+          store_no_shadow s ->
+          root_env_no_shadow R ->
+          store_frame_scope ps Σ s frame ->
+          store_frame_static_fresh Σ frame ->
+          store_param_scope ps s frame ->
+          store_frame_scope ps Σ' s' frame /\
+          exists frame', store_param_scope ps s' frame').
+Proof.
+  intros Htyping_prefix Hprefix_ready Hroots_ready Hroot_names Hroot_keys
+    Hstatic Hframe_ready Hparam_ready base_env base_fname Htarget_provider
+    Hprovider.
+  assert (Hall : forall n_call,
+    (forall env fname,
+      store_safe_synthetic_direct_call_ready_exact_body_call_route_reachable
+        base_env base_fname env fname ->
+      forall s args s' v,
+        eval env s (ECall fname args) s' v ->
+        direct_call_eval_height env s (ECall fname args) s' v n_call ->
+        forall (Omega : outlives_ctx) (n : nat) R Σ T Σ' R' roots,
+          preservation_ready_args args ->
+          store_typed_prefix env s Σ ->
+          store_roots_within R s ->
+          store_no_shadow s ->
+          root_env_no_shadow R ->
+          root_env_store_roots_named R s ->
+          root_env_store_keys_named R s ->
+          typed_env_roots env Omega n R Σ (ECall fname args) T Σ' R'
+            roots ->
+          fn_env_unique_by_name env ->
+          fn_root_shadow_synthetic_direct_call_ready_summary_evidence_at env
+            fname ->
+          direct_call_callee_body_root_synthetic_direct_call_ready_evidence_at
+            env fname ->
+          store_typed_prefix env s' Σ' /\
+          value_has_type env s' v T /\
+          store_ref_targets_preserved env s s' /\
+          store_roots_within R' s' /\
+          value_roots_within roots v /\
+          store_no_shadow s' /\
+          root_env_no_shadow R') /\
+    (forall env fname,
+      store_safe_synthetic_direct_call_ready_exact_body_call_route_reachable
+        base_env base_fname env fname ->
+      forall s args s' v,
+        eval env s (ECall fname args) s' v ->
+        direct_call_eval_height env s (ECall fname args) s' v n_call ->
+        forall (Omega : outlives_ctx) (n : nat) R Σ T Σ' R' roots ps frame,
+          preservation_ready_args args ->
+          store_typed_prefix env s Σ ->
+          root_env_store_roots_named R s ->
+          root_env_store_keys_named R s ->
+          typed_env_roots env Omega n R Σ (ECall fname args) T Σ' R'
+            roots ->
+          fn_env_unique_by_name env ->
+          fn_root_shadow_synthetic_direct_call_ready_summary_evidence_at env
+            fname ->
+          direct_call_callee_body_root_synthetic_direct_call_ready_evidence_at
+            env fname ->
+          root_env_covers_params ps R ->
+          store_roots_within R s ->
+          store_no_shadow s ->
+          root_env_no_shadow R ->
+          store_frame_scope ps Σ s frame ->
+          store_frame_static_fresh Σ frame ->
+          store_param_scope ps s frame ->
+          store_frame_scope ps Σ' s' frame /\
+          exists frame', store_param_scope ps s' frame')).
+  { intro n_call.
+    induction n_call as [n_call IH] using Wf_nat.lt_wf_ind.
+    split.
+    - intros env fname Hreachable s args s' v Heval Hheight Omega n R Σ T
+        Σ' R' roots Hready Hstore Hroots Hshadow Hrn Hnamed Hkeys Htyped
+        Hunique Hsummary Hevidence.
+      eapply eval_preserves_typing_roots_synthetic_direct_call_ready_summary_at_prefix_call_height_statement_evidence_at_current_from_reachable_less_callbacks_and_exact_body_call_route_package_and_target_provider;
+        try eassumption.
+      + intros m Hlt env0 fname0 Hreachable0 s0 args0 s0' v0 Heval0
+          Hheight0 Omega0 n0 R0 Σ0 T0 Σ0' R0' roots0 Hready0 Hstore0
+          Hroots0 Hshadow0 Hrn0 Hnamed0 Hkeys0 Htyped0 Hunique0 Hsummary0
+          Hevidence0.
+        exact (proj1 (IH m Hlt) env0 fname0 Hreachable0 s0 args0 s0' v0
+          Heval0 Hheight0 Omega0 n0 R0 Σ0 T0 Σ0' R0' roots0 Hready0
+          Hstore0 Hroots0 Hshadow0 Hrn0 Hnamed0 Hkeys0 Htyped0 Hunique0
+          Hsummary0 Hevidence0).
+      + intros m Hlt env0 fname0 Hreachable0 s0 args0 s0' v0 Heval0
+          Hheight0 Omega0 n0 R0 Σ0 T0 Σ0' R0' roots0 ps0 frame0
+          Hready0 Hstore0 Hnamed0 Hkeys0 Htyped0 Hunique0 Hsummary0
+          Hevidence0 Hcover0 Hroots0 Hshadow0 Hrn0 Hframe0 Hfresh0
+          Hparam0.
+        exact (proj2 (IH m Hlt) env0 fname0 Hreachable0 s0 args0 s0' v0
+          Heval0 Hheight0 Omega0 n0 R0 Σ0 T0 Σ0' R0' roots0 ps0 frame0
+          Hready0 Hstore0 Hnamed0 Hkeys0 Htyped0 Hunique0 Hsummary0
+          Hevidence0 Hcover0 Hroots0 Hshadow0 Hrn0 Hframe0 Hfresh0
+          Hparam0).
+    - intros env fname Hreachable s args s' v Heval Hheight Omega n R Σ T
+        Σ' R' roots ps frame Hready Hstore Hnamed Hkeys Htyped Hunique
+        Hsummary Hevidence Hcover Hroots Hshadow Hrn Hframe Hfresh Hparam.
+      eapply eval_preserves_frame_param_scope_synthetic_direct_call_ready_summary_at_prefix_call_height_statement_evidence_at_current_from_reachable_less_callbacks_and_exact_body_call_route_package_and_target_provider;
+        try eassumption.
+      + intros m Hlt env0 fname0 Hreachable0 s0 args0 s0' v0 Heval0
+          Hheight0 Omega0 n0 R0 Σ0 T0 Σ0' R0' roots0 Hready0 Hstore0
+          Hroots0 Hshadow0 Hrn0 Hnamed0 Hkeys0 Htyped0 Hunique0 Hsummary0
+          Hevidence0.
+        exact (proj1 (IH m Hlt) env0 fname0 Hreachable0 s0 args0 s0' v0
+          Heval0 Hheight0 Omega0 n0 R0 Σ0 T0 Σ0' R0' roots0 Hready0
+          Hstore0 Hroots0 Hshadow0 Hrn0 Hnamed0 Hkeys0 Htyped0 Hunique0
+          Hsummary0 Hevidence0).
+      + intros m Hlt env0 fname0 Hreachable0 s0 args0 s0' v0 Heval0
+          Hheight0 Omega0 n0 R0 Σ0 T0 Σ0' R0' roots0 ps0 frame0
+          Hready0 Hstore0 Hnamed0 Hkeys0 Htyped0 Hunique0 Hsummary0
+          Hevidence0 Hcover0 Hroots0 Hshadow0 Hrn0 Hframe0 Hfresh0
+          Hparam0.
+        exact (proj2 (IH m Hlt) env0 fname0 Hreachable0 s0 args0 s0' v0
+          Heval0 Hheight0 Omega0 n0 R0 Σ0 T0 Σ0' R0' roots0 ps0 frame0
+          Hready0 Hstore0 Hnamed0 Hkeys0 Htyped0 Hunique0 Hsummary0
+          Hevidence0 Hcover0 Hroots0 Hshadow0 Hrn0 Hframe0 Hfresh0
+          Hparam0). }
+  split.
+  - intros env fname Hreachable s args s' v n_call Heval Hheight Omega n R
+      Σ T Σ' R' roots Hready Hstore Hroots Hshadow Hrn Hnamed Hkeys Htyped
+      Hunique Hsummary Hevidence.
+    exact (proj1 (Hall n_call) env fname Hreachable s args s' v Heval
+      Hheight Omega n R Σ T Σ' R' roots Hready Hstore Hroots Hshadow Hrn
+      Hnamed Hkeys Htyped Hunique Hsummary Hevidence).
+  - intros env fname Hreachable s args s' v n_call Heval Hheight Omega n R
+      Σ T Σ' R' roots ps frame Hready Hstore Hnamed Hkeys Htyped Hunique
+      Hsummary Hevidence Hcover Hroots Hshadow Hrn Hframe Hfresh Hparam.
+    exact (proj2 (Hall n_call) env fname Hreachable s args s' v Heval
+      Hheight Omega n R Σ T Σ' R' roots ps frame Hready Hstore Hnamed Hkeys
+      Htyped Hunique Hsummary Hevidence Hcover Hroots Hshadow Hrn Hframe
+      Hfresh Hparam).
+Qed.
+
 Theorem eval_preserves_typing_roots_store_safe_synthetic_direct_call_ready_body_call_store_safe_callback_height_statement_at_of_reachable_exact_body_call_route_package_provider :
   eval_preserves_typing_ready_prefix_mutual_statement ->
   eval_preserves_typing_roots_ready_prefix_mutual_statement ->
@@ -13146,6 +14049,53 @@ Proof.
     (eval_preserves_typing_roots_and_frame_param_scope_synthetic_direct_call_ready_summary_at_prefix_call_height_statement_evidence_at_of_reachable_exact_body_call_route_package_provider
       Htyping_prefix Hprefix_ready Hroots_ready Hroot_names Hroot_keys Hstatic
       Hframe_ready Hparam_ready Hexact_body_target base_env base_fname
+      Hprovider) as Hroute.
+  destruct Hroute as [Htyping_route _Hscope_route].
+  unfold
+    eval_preserves_typing_roots_store_safe_synthetic_direct_call_ready_body_call_store_safe_callback_height_statement_at.
+  intros fname fcall used used' s_args s_body vs ret R_args arg_roots
+    fname_body args_body T_body Gamma_out R_body roots_body Hin Hname
+    Hrename Htarget Hsafe_args Hready Htyped Hunique Hsummary Hevidence
+    Hstore Hroots Hshadow Hrn Hnamed Hkeys Heval n_body_call Hheight.
+  assert (Hreachable_body :
+    store_safe_synthetic_direct_call_ready_exact_body_call_route_reachable
+      base_env base_fname
+      (global_env_with_local_bounds base_env (fn_bounds fcall)) fname_body).
+  { eapply store_safe_synthetic_direct_call_ready_exact_body_call_route_reachable_body_call_step.
+    - constructor.
+    - exact Hin_base.
+    - exact Hname_base.
+    - exact Hrename.
+    - exact Htarget. }
+  eapply Htyping_route; try eassumption.
+Qed.
+
+Theorem eval_preserves_typing_roots_store_safe_synthetic_direct_call_ready_body_call_store_safe_callback_height_statement_at_of_reachable_exact_body_call_route_package_and_target_provider :
+  eval_preserves_typing_ready_prefix_mutual_statement ->
+  eval_preserves_typing_roots_ready_prefix_mutual_statement ->
+  eval_preserves_roots_ready_mutual_statement ->
+  eval_preserves_root_names_ready_mutual_statement ->
+  eval_preserves_root_keys_named_ready_mutual_statement ->
+  preservation_ready_expr_static_runtime_named_statement ->
+  eval_preserves_frame_scope_roots_ready_mutual_statement ->
+  eval_preserves_param_scope_roots_ready_mutual_statement ->
+  forall base_env base_fname fdef,
+    store_safe_synthetic_direct_call_ready_exact_body_call_route_reachable_exact_body_target_provider
+      base_env base_fname ->
+    store_safe_synthetic_direct_call_ready_exact_body_call_route_reachable_package_provider
+      base_env base_fname ->
+    In fdef (env_fns base_env) ->
+    fn_name fdef = base_fname ->
+    eval_preserves_typing_roots_store_safe_synthetic_direct_call_ready_body_call_store_safe_callback_height_statement_at
+      base_env fdef.
+Proof.
+  intros Htyping_prefix Hprefix_ready Hroots_ready Hroot_names Hroot_keys
+    Hstatic Hframe_ready Hparam_ready base_env base_fname fdef
+    Htarget_provider Hprovider Hin_base Hname_base.
+  pose proof
+    (eval_preserves_typing_roots_and_frame_param_scope_synthetic_direct_call_ready_summary_at_prefix_call_height_statement_evidence_at_of_reachable_exact_body_call_route_package_and_target_provider
+      Htyping_prefix Hprefix_ready Hroots_ready Hroot_names Hroot_keys Hstatic
+      Hframe_ready Hparam_ready base_env base_fname Htarget_provider
       Hprovider) as Hroute.
   destruct Hroute as [Htyping_route _Hscope_route].
   unfold
